# HW2
11811126 庄宇伦
## 1.
### (a)
$$
\bm{x(k+1)}= 
\left[
\begin{matrix}
   x_1(k) \\
   max(x_1(k),x_2(k),x_3(k)) \\
   max(x_1(k),x_3(k),x_4(k)) \\
   max(x_4(k),x_5(k)) \\
   max(x_2(k),x_5(k)) \\
\end{matrix}
\right]
$$
### (b) 
$$
\bm{x(k+1)}=
\begin{bmatrix}
    1&0&0&0&0\\
    1/3&1/3&1/3&0&0\\
    1/3&0&1/3&1/3&0\\
    0&0&0&1/2&1/2\\
    0&1/2&0&0&1/2
\end{bmatrix}
\begin{bmatrix}
    x_1(k)\\
    x_2(k)\\
    x_3(k)\\
    x_4(k)\\
    x_5(k)\\
\end{bmatrix}
$$
## 2
### (a)
$$
\left\{
\begin{aligned}
    f_y&=mg\\
    f_x&=m\ddot{x_m}\\
    \frac{f_x}{f_y}&=\frac{x_m-x_p}{h}
\end{aligned}
\right.\\
\Rightarrow
h\ddot{x_m}=gx_m-gx_p\\
$$
## (b)
$$
\begin{aligned}
\bm{x}&=
\begin{bmatrix}
    x_m\\\dot{x_m}
\end{bmatrix}
\\
\bm{\dot{x}}&=
\begin{bmatrix}
    0&1\\g/h&0
\end{bmatrix}
\begin{bmatrix}
    x_m\\\dot{x_m}
\end{bmatrix}
+
\begin{bmatrix}
    0&-g/h
\end{bmatrix}
x_p\\
\Rightarrow
\\
A&=
\begin{bmatrix}
    0&1\\g/h&0
\end{bmatrix}
\\
B&=
\begin{bmatrix}
    0&-g/h
\end{bmatrix}
\end{aligned}
$$
## 3
### (a)
$$
\begin{aligned}
\bm{x}&=
\begin{bmatrix}
    x_1\\x_2
\end{bmatrix}
,y=x_1
\\
where\ x_1&=i_L,\ x_2=v_C
\\
&\left\{
    \begin{aligned}
    i_L&=i_C+i_R\\
    v_g&=v_L+v_C\\
    v_L&=L\dot{i_L}\\
    i_C&=C\dot{v_C}\\
    i_R&=v_C/R
    \end{aligned}   
\right.
\\
\Rightarrow\\
\bm{\dot{x}}&=
\begin{bmatrix}
    0&-1/L\\1/C&-1/RC
\end{bmatrix}
\begin{bmatrix}
    x_1\\x_2
\end{bmatrix}
+
\begin{bmatrix}
    1/L\\0
\end{bmatrix}
v_g\\
\bm{y}&=
\begin{bmatrix}
    0&1
\end{bmatrix}
\bm{x}
\end{aligned}
$$
### (b)
$$
\begin{aligned}
\bm{x}&=
\begin{bmatrix}
    x_1\\x_2
\end{bmatrix}
,y=x_1
\\
where\ x_1&=i_L,\ x_2=v_C
\\
&\left\{
    \begin{aligned}
    i_L&=i_C+i_R\\
    0&=v_L+v_C\\
    v_L&=L\dot{i_L}\\
    i_C&=C\dot{v_C}\\
    i_R&=v_C/R
    \end{aligned}   
\right.
\\
\Rightarrow\\
\bm{\dot{x}}&=
\begin{bmatrix}
    0&-1/L\\1/C&-1/RC
\end{bmatrix}
\begin{bmatrix}
    x_1\\x_2
\end{bmatrix}
\\
\bm{y}&=
\begin{bmatrix}
    0&1
\end{bmatrix}
\bm{x}
\end{aligned}
$$
## 4
$$
\begin{aligned}
&L\dot{i_a}+Ri_a=v_a-K_b\dot{\theta_m}\\
&J_m\ddot{\theta_m}+B\dot{\theta_m}=K_mi_a-\tau_l/r\\
&let\ x_1=\theta_m,x_2=\dot{\theta_m},x_3=i_a\\
\bm{\dot{x}}&=
\begin{bmatrix}
    0&1&0\\
    0&-B/J_m&K_m/J_m\\
    0&-K_b/L&-R/L
\end{bmatrix}
\bm{x}
+
\begin{bmatrix}
    0\\0\\1/L
\end{bmatrix}
v_a
+
\begin{bmatrix}
    0\\-1/(J_mr)
\end{bmatrix}
\tau_l\\
\bm{y}&=
\begin{bmatrix}
    1&0&0
\end{bmatrix}
\bm{x}
\end{aligned}
$$
## 5
### (a)
$$
\begin{aligned}
ml^2\ddot{\theta}&+mgl\sin{\theta}-bl^2\dot{\theta}=0
\\
\bm{x}&=
\begin{bmatrix}
    x_1\\x_2
\end{bmatrix}
,y=x_1
\\
where\ x_1&=\theta,\ x_2=\dot{\theta}\\
\\\Rightarrow\\
\bm{\dot{x}}&=
\begin{bmatrix}
    x_2\\
    -\frac{gsinx_1}{l}-\frac{bx_2}{m}
\end{bmatrix}\\
\bm{y}&=
\begin{bmatrix}
    x_1
\end{bmatrix}
\end{aligned}
$$

### (b)

$$
\begin{aligned}
\bm{\hat{x}}&=
\begin{bmatrix}
    0\\0
\end{bmatrix}
\\
\hat{A}&=
\left.
\frac{\partial f}{\partial x}
\right|_{\hat{x}}
=
\begin{bmatrix}
    0&1\\
    -g/l&-b/m
\end{bmatrix}\\
\hat{C}&=
\left .
\frac{\partial h}{\partial x}
\right|_{\hat{x}}
=
\begin{bmatrix}
    1&0
\end{bmatrix}
\end{aligned}
$$

### (c)

$$
\begin{aligned}
\bm{x(k+1)}&=\bm{x(k)}+A_d\bm{x(k)}\Delta t
\\
where\ A_d&=\hat{A},\ \Delta t=2\\
\Rightarrow\\
\bm{x(k+1)}&=
\begin{bmatrix}
    1&2\\-2g/l&1-2b/m
\end{bmatrix}
\bm{x(k)}\\
\bm{y(k)}&=
\begin{bmatrix}
    1&0
\end{bmatrix}
\bm{x(k)}\\
\end{aligned}
$$
